crypto/bignum/Hacl.Spec.Bignum.Fdifference.fst
@@ -1,7 +1,7 @@
 module Hacl.Spec.Bignum.Fdifference
 
 open Hacl.Bignum.Parameters
-open Hacl.Bignum.Bigint
+open Hacl.Spec.Bignum.Bigint
 open Hacl.Bignum.Limb
 
 module U32 = FStar.UInt32
