crypto/bignum/interfaces/Hacl.Bignum.Crecip.fsti
@@ -5,7 +5,7 @@ open FStar.HyperStack
 open FStar.Buffer
 
 open Hacl.Bignum.Parameters
-open Hacl.Bignum.Bigint
+open Hacl.Spec.Bignum.Bigint
 open Hacl.Bignum.Limb
 
 module U32 = FStar.UInt32
