crypto/bignum/interfaces/Hacl.EC.Point.fsti
@@ -6,7 +6,7 @@ open FStar.Ghost
 open FStar.Buffer
 
 open Hacl.Bignum.Parameters
-open Hacl.Bignum.Bigint
+open Hacl.Spec.Bignum.Bigint
 open Hacl.Bignum.Limb
 open Hacl.Bignum
 
