crypto/bignum/interfaces/Hacl.Spec.Bignum.Modulo.fsti
@@ -7,7 +7,7 @@ open FStar.Buffer
 
 open Hacl.Bignum.Constants
 open Hacl.Bignum.Parameters
-open Hacl.Bignum.Bigint
+open Hacl.Spec.Bignum.Bigint
 open Hacl.Bignum.Limb
 
 
