crypto/bignum/poly1305/Hacl.Spec.Bignum.Fmul.Lemmas.fst
@@ -2,7 +2,7 @@ module Hacl.Spec.Bignum.Fmul.Lemmas
 
 open Hacl.Bignum.Constants
 open Hacl.Bignum.Parameters
-open Hacl.Bignum.Bigint
+open Hacl.Spec.Bignum.Bigint
 open Hacl.Bignum.Limb
 
 open Hacl.Spec.Bignum.Modulo
