crypto/bignum/x25519/Hacl.Bignum.Crecip.fst
@@ -4,7 +4,7 @@ open FStar.HyperStack
 open FStar.Buffer
 
 open Hacl.Bignum.Parameters
-open Hacl.Bignum.Bigint
+open Hacl.Spec.Bignum.Bigint
 open Hacl.Bignum.Limb
 open Hacl.Bignum.Fmul
 
