crypto/bignum/x25519/Hacl.Bignum.Modulo.fst
@@ -5,7 +5,7 @@ open FStar.HyperStack
 open FStar.Buffer
 
 open Hacl.Bignum.Parameters
-open Hacl.Bignum.Bigint
+open Hacl.Spec.Bignum.Bigint
 open Hacl.Bignum.Limb
 open Hacl.Spec.Bignum.Modulo
 
@@ -18,6 +18,13 @@ inline_for_extraction let mask_51    =
   assert_norm (0x7ffffffffffff < pow2 64);uint64_to_limb 0x7ffffffffffffuL
 
 
+val add_zero:
+  b:felem ->
+  Stack unit
+    (requires (fun h -> live h b /\ add_zero_pre (as_seq h b)))
+    (ensures (fun h0 _ h1 -> live h0 b /\ add_zero_pre (as_seq h0 b) /\ live h1 b /\ modifies_1 b h0 h1
+      /\ as_seq h1 b == add_zero_spec (as_seq h0 b)
+      /\ eval h1 b % prime = eval h0 b % prime))
 let add_zero b =
   let b0 = b.(0ul) in
   let b1 = b.(1ul) in
@@ -31,6 +38,12 @@ let add_zero b =
   b.(4ul) <- b4 +^ two54m8
 
 
+val carry_top:
+  b:felem ->
+  Stack unit
+  (requires (fun h -> live h b /\ carry_top_pre (as_seq h b)))
+  (ensures (fun h0 _ h1 -> live h0 b /\ carry_top_pre (as_seq h0 b) /\ live h1 b /\ modifies_1 b h0 h1
+    /\ as_seq h1 b == carry_top_spec (as_seq h0 b)))
 let carry_top b =
   let b4 = b.(4ul) in
   let b0 = b.(0ul) in
@@ -42,12 +55,24 @@ let carry_top b =
   b.(0ul) <- b0'
 
 
+val reduce:
+  b:felem ->
+  Stack unit
+  (requires (fun h -> live h b /\ reduce_pre (as_seq h b)))
+  (ensures (fun h0 _ h1 -> live h0 b /\ reduce_pre (as_seq h0 b) /\ live h1 b /\ modifies_1 b h0 h1
+    /\ as_seq h1 b == reduce_spec (as_seq h0 b)))
 let reduce b =
   let nineteen = (limb_one <<^ 4ul) +^ (limb_one <<^ 1ul) +^ limb_one in
   let b0 = b.(0ul) in
   b.(0ul) <- nineteen *^ b0
 
 
+val carry_top_wide:
+  b:felem_wide ->
+  Stack unit
+    (requires (fun h -> live h b /\ carry_top_wide_pre (as_seq h b)))
+    (ensures (fun h0 _ h1 -> live h0 b /\ carry_top_wide_pre (as_seq h0 b) /\ live h1 b /\ modifies_1 b h0 h1
+      /\ as_seq h1 b == carry_top_wide_spec (as_seq h0 b)))
 let carry_top_wide b =
   let b4 = b.(4ul) in
   let b0 = b.(0ul) in
