crypto/bignum/x25519/Hacl.EC.Point.fst
@@ -6,7 +6,7 @@ open FStar.Ghost
 open FStar.Buffer
 
 open Hacl.Bignum.Parameters
-open Hacl.Bignum.Bigint
+open Hacl.Spec.Bignum.Bigint
 open Hacl.Bignum.Limb
 open Hacl.Bignum
 
@@ -15,28 +15,40 @@ module U32 = FStar.UInt32
 (* let plen = 10 *)
 (* let cplen = 10ul *)
 
+val point : Type0
 let point =
   let _ = () in
   b:buffer limb{length b = 10}
 
+
+(** Coordinate getters *)
+val getx: point -> Tot felem
+val gety: point -> Tot felem
+val getz: point -> Tot felem
 let getx p = Buffer.sub p 0ul 5ul
 let gety p = Buffer.sub p 0ul 5ul
 let getz p = Buffer.sub p 5ul 5ul
 
+val live_coords: mem -> felem -> felem -> felem -> GTot Type0
 let live_coords h x y z =
   let _ = () in
   live h x /\ live h z
 
+val live: mem -> point -> GTot Type0
 let live h p =
   let _ = () in
   live_coords h (getx p) (gety p) (getz p)
 
+val make_pre: x:felem -> y:felem -> z:felem -> GTot Type0
 let make_pre x y z =
   let _ = () in
   content x == content z /\ max_length x == max_length z /\ idx z = idx x + length x
 
+val make: x:felem -> y:felem -> z:felem{make_pre x y z} -> Tot (p:point)
 let make x y z = join x z
 
+(** Workable state of a point **)
+val valid: mem -> point -> GTot bool
 let valid h p = admit()
 
 
@@ -58,11 +70,24 @@ private let rec swap_conditional_ a b swap ctr =
     swap_conditional_ a b swap i
   )
 
+val swap_conditional:
+  a:point ->
+  b:point ->
+  i:limb ->
+  Stack unit
+    (requires (fun _ -> true))
+    (ensures (fun _ _ _ -> true))
 let swap_conditional a b iswap =
   let swap = limb_zero -%^ iswap in
   swap_conditional_ (getx a) (getx b) swap clen;
   swap_conditional_ (getz a) (getz b) swap clen
 
+val copy:
+  output:point ->
+  input:point ->
+  Stack unit
+    (requires (fun _ -> true))
+    (ensures (fun _ _ _ -> true))
 let copy output input =
   blit (getx input) 0ul (getx output) 0ul clen;
   blit (getz input) 0ul (getz output) 0ul clen
